theories/VLSM/Core/Composition.v
@@ -1429,7 +1429,9 @@ Definition same_IM_state_rew
   : composite_state IM2 :=
   fun i => same_VLSM_state_rew (Heq i) (s1 i).
 
-Section pre_loaded_constrained.
+Definition same_IM_sym : forall i, IM2 i = IM1 i := fun i => eq_sym (Heq i).
+
+Section sec_same_IM_constrained.
 
 Context
   (constraint1 : composite_label IM1 -> composite_state IM1 * option message -> Prop)
@@ -1438,10 +1440,15 @@ Context
     : forall s1, valid_state_prop (pre_loaded_with_all_messages_vlsm (free_composite_vlsm IM1)) s1 ->
       forall l1 om, constraint1 l1 (s1,om) ->
     constraint2 (same_IM_label_rew l1) (same_IM_state_rew s1, om))
+  .
+
+Section sec_same_IM_preloaded_full_projection.
+
+Context
   (seed : message -> Prop)
   .
 
-Lemma same_IM_full_projection
+Lemma same_IM_preloaded_full_projection
   : VLSM_full_projection
     (pre_loaded_vlsm (composite_vlsm IM1 constraint1) seed)
     (pre_loaded_vlsm (composite_vlsm IM2 constraint2) seed)
@@ -1478,7 +1485,28 @@ Proof.
     + exists (exist _ m Hm). reflexivity.
 Qed.
 
-End pre_loaded_constrained.
+End sec_same_IM_preloaded_full_projection.
+
+Lemma same_IM_full_projection
+  : VLSM_full_projection
+    (composite_vlsm IM1 constraint1)
+    (composite_vlsm IM2 constraint2)
+    same_IM_label_rew
+    same_IM_state_rew.
+Proof.
+  constructor.
+  intros s1 tr1 Htr1.
+  apply
+    (VLSM_eq_finite_valid_trace
+      (vlsm_is_pre_loaded_with_False (composite_vlsm IM2 constraint2))),
+    (VLSM_full_projection_finite_valid_trace
+      (same_IM_preloaded_full_projection (fun _ => False))),
+    (VLSM_eq_finite_valid_trace
+      (vlsm_is_pre_loaded_with_False (composite_vlsm IM1 constraint1))).
+  assumption.
+Qed.
+
+End sec_same_IM_constrained.
 
 Lemma same_IM_preloaded_free_full_projection
   : VLSM_full_projection
@@ -1489,16 +1517,16 @@ Lemma same_IM_preloaded_free_full_projection
 Proof.
   constructor.
   intros s1 tr1 Htr1.
-  specialize (pre_loaded_with_all_messages_vlsm_is_pre_loaded_with_True (free_composite_vlsm IM1)) as Heq1.
-  apply (VLSM_eq_finite_valid_trace Heq1) in Htr1.
-  clear Heq1.
-  specialize (same_IM_full_projection (free_constraint IM1) (free_constraint IM2))
+  specialize (same_IM_preloaded_full_projection (free_constraint IM1) (free_constraint IM2))
     as Hproj.
-  spec Hproj. { intros. exact I. }
+  spec Hproj; [intros; exact I|].
   specialize (Hproj (fun _ => True)).
-  apply (VLSM_full_projection_finite_valid_trace Hproj) in Htr1.
-  specialize (pre_loaded_with_all_messages_vlsm_is_pre_loaded_with_True (free_composite_vlsm IM2)) as Heq2.
-  apply (VLSM_eq_finite_valid_trace Heq2).
+  apply
+    (VLSM_eq_finite_valid_trace
+      (pre_loaded_with_all_messages_vlsm_is_pre_loaded_with_True (free_composite_vlsm IM2))),
+    (VLSM_full_projection_finite_valid_trace Hproj),
+    (VLSM_eq_finite_valid_trace
+      (pre_loaded_with_all_messages_vlsm_is_pre_loaded_with_True (free_composite_vlsm IM1))).
   assumption.
 Qed.
 
@@ -1506,3 +1534,26 @@ End sec_same_IM_full_projection.
 
 Arguments same_IM_label_rew {_ _ _ _} _ _ : assert.
 Arguments same_IM_state_rew {_ _ _ _} _ _ _ : assert.
+Arguments same_IM_sym {_ _ _ _} _ _ : assert.
+
+Lemma same_IM_state_rew_12
+  {message : Type}
+  `{EqDecision index}
+  {IM1 IM2 : index -> VLSM message}
+  (Heq : forall i, IM1 i = IM2 i)
+  : forall s : composite_state IM1,
+    same_IM_state_rew (same_IM_sym Heq) (same_IM_state_rew Heq s) = s.
+Proof.
+  intro; extensionality i; apply same_VLSM_state_rew_12.
+Qed.
+
+Lemma same_IM_state_rew_21
+  {message : Type}
+  `{EqDecision index}
+  {IM1 IM2 : index -> VLSM message}
+  (Heq : forall i, IM1 i = IM2 i)
+  : forall s : composite_state IM2,
+    same_IM_state_rew Heq (same_IM_state_rew (same_IM_sym Heq) s) = s.
+Proof.
+  intro; extensionality i; apply same_VLSM_state_rew_21.
+Qed.
